Unicode/Generated/BIP39/English.lean
@@ -11,7 +11,7 @@ namespace Unicode.Generated.BIP39.English
 set_option maxRecDepth 100000
 
 /-- The 2,048 words in canonical BIP-39 order. -/
-def wordlist : Array String := #[
+def wordlist : List String := [
   "abandon",
   "ability",
   "able",
@@ -2062,7 +2062,7 @@ def wordlist : Array String := #[
   "zoo"
 ]
 
-theorem wordlist_count : wordlist.size = 2048 := by decide
+theorem wordlist_count : wordlist.length = 2048 := by decide
 
 theorem first_word : wordlist[0]! = "abandon" := by decide
 
